SelAddrSLH.v
@@ -1,0 +1,252 @@
+(** * aSelSLH : Selective Address SLH *)
+
+(* TERSE: HIDEFROMHTML *)
+Set Warnings "-notation-overridden,-parsing,-deprecated-hint-without-locality".
+From Coq Require Import Strings.String.
+From SECF Require Import Maps SpecCT UltimateSLH_optimized.
+From Coq Require Import Bool.Bool.
+From Coq Require Import Arith.Arith.
+From Coq Require Import Arith.EqNat.
+From Coq Require Import Arith.PeanoNat. Import Nat.
+From Coq Require Import Lia.
+From Coq Require Import List. Import ListNotations.
+Set Default Goal Selector "!".
+(* TERSE: /HIDEFROMHTML *)
+
+Ltac rewrite_eq :=
+  match goal with
+  | H:_=_ |- _ => rewrite H; clear H
+  | H:forall _, _=_ |- _ => rewrite H; clear H
+  | _ => idtac
+ end.
+
+Fixpoint label_of_aexp (P:pub_vars) (a:aexp) : label :=
+  match a with
+  | ANum n => public
+  | AId x => P x
+  | <{ a1 + a2 }>
+  | <{ a1 - a2 }>
+  | <{ a1 * a2 }> => join (label_of_aexp P a1) (label_of_aexp P a2)
+  | <{ be ? a1 : a2 }> => join (label_of_bexp P be) (join (label_of_aexp P a1) (label_of_aexp P a2))
+  end
+with label_of_bexp (P:pub_vars) (b:bexp) : label :=
+  match b with
+  | <{ true }> | <{ false }> => public
+  | <{ a1 = a2 }>
+  | <{ a1 <> a2 }>
+  | <{ a1 <= a2 }>
+  | <{ a1 > a2 }> => join (label_of_aexp P a1) (label_of_aexp P a2)
+  | <{ ~b }> => label_of_bexp P b
+  | <{ b1 && b2 }> => join (label_of_bexp P b1) (label_of_bexp P b2)
+  end.
+
+Lemma label_of_exp_sound : forall P,
+  (forall a, P |-a- a \in label_of_aexp P a) /\
+  (forall b, P |-b- b \in label_of_bexp P b).
+Proof. intro P. apply aexp_bexp_mutind; intros; now constructor. Qed.
+
+Corollary label_of_aexp_sound : forall P a,
+  P |-a- a \in label_of_aexp P a.
+Proof. intros. apply label_of_exp_sound. Qed.
+
+Corollary label_of_bexp_sound : forall P b,
+  P |-b- b \in label_of_bexp P b.
+Proof. intros. apply label_of_exp_sound. Qed.
+
+Lemma label_of_exp_unique : forall P,
+  (forall a l, P |-a- a \in l -> l = label_of_aexp P a) /\
+  (forall b l, P |-b- b \in l -> l = label_of_bexp P b).
+Proof. intro P. apply aexp_bexp_has_label_mutind; intros; (repeat rewrite_eq); reflexivity. Qed.
+
+Corollary label_of_aexp_unique : forall P a l,
+  P |-a- a \in l ->
+  l = label_of_aexp P a.
+Proof. intro. apply label_of_exp_unique. Qed.
+
+Corollary label_of_bexp_unique : forall P b l,
+  P |-b- b \in l ->
+  l = label_of_bexp P b.
+Proof. intro. apply label_of_exp_unique. Qed.
+
+Corollary aexp_has_label_inj : forall P a l l',
+  P |-a- a \in l ->
+  P |-a- a \in l' ->
+  l = l'.
+Proof. intros. apply label_of_aexp_unique in H, H0. now rewrite_eq. Qed.
+
+Corollary bexp_has_label_inj : forall P b l l',
+  P |-b- b \in l ->
+  P |-b- b \in l' ->
+  l = l'.
+Proof. intros. apply label_of_bexp_unique in H, H0. now rewrite_eq. Qed.
+
+Fixpoint addr_sel_slh (P : pub_vars) (c : com) : com :=
+  (match c with
+  | <{{ skip }}> => <{{ skip }}>
+  | <{{ x := e }}> => <{{ x := e }}>
+  | <{{ c1; c2 }}> => <{{ addr_sel_slh P c1; addr_sel_slh P c2 }}>
+  | <{{ if b then c1 else c2 end }}> => <{{ if b then "b" := (b ? "b" : 1); addr_sel_slh P c1 else
+                                                  "b" := (b ? 1 : "b"); addr_sel_slh P c2 end }}>
+  | <{{ while b do c end }}> => <{{ while b do "b" := (b ? "b" : 1); addr_sel_slh P c end; "b" := b ? 1 : "b" }}>
+  | <{{ x <- a [[ i ]] }}> => let i' := if P x then <{ ("b" = 0) ? i : 0 }> else i in
+                              <{{ x <- a [[ i' ]] }}>
+  | <{{ a [ i ] <- e }}> => let i' := if label_of_aexp P e then i else <{ ("b" = 0) ? i : 0 }> in
+                            <{{ a [ i' ] <- e }}>
+  end)%string.
+
+(** * Ideal small-step evaluation *)
+
+Reserved Notation
+  "P '|-' '<((' c , st , ast , b '))>' '-->i_' ds '^^' os '<((' ct , stt , astt , bt '))>'"
+  (at level 40, c custom com at level 99, ct custom com at level 99,
+   st constr, ast constr, stt constr, astt constr at next level).
+
+Inductive ideal_eval_small_step :
+    pub_vars -> com -> state -> astate -> bool ->
+    com -> state -> astate -> bool -> dirs -> obs -> Prop :=
+  | ISM_Asgn  : forall P st ast b e n x,
+      aeval st e = n ->
+      P |- <((x := e, st, ast, b))> -->i_[]^^[] <((skip, x !-> n; st, ast, b))>
+  | ISM_Seq : forall P c1 st ast b ds os c1t stt astt bt c2,
+      P |- <((c1, st, ast, b))>  -->i_ds^^os <((c1t, stt, astt, bt))>  ->
+      P |- <(((c1;c2), st, ast, b))>  -->i_ds^^os <(((c1t;c2), stt, astt, bt))>
+  | ISM_Seq_Skip : forall P st ast b c2,
+      P |- <(((skip;c2), st, ast, b))>  -->i_[]^^[] <((c2, st, ast, b))>
+  | ISM_If : forall P be ct cf st ast b b' c',
+      b' = beval st be ->
+      c' = (if b' then ct else cf) ->
+      P |- <((if be then ct else cf end, st, ast, b))> -->i_[DStep]^^[OBranch b'] <((c', st, ast, b))>
+  | ISM_If_F : forall P be ct cf st ast b b' c',
+      b' = beval st be ->
+      c' = (if b' then cf else ct) ->
+      P |- <((if be then ct else cf end, st, ast, b))> -->i_[DForce]^^[OBranch b'] <((c', st, ast, true))>
+  | ISM_While : forall P be c st ast b,
+      P |- <((while be do c end, st, ast, b))> -->i_[]^^[]
+            <((if be then c; while be do c end else skip end, st, ast, b))>
+  | ISM_ARead : forall P x a ie st ast (b :bool) i,
+      (if P x && b then 0 else (aeval st ie)) = i ->
+      i < length (ast a) ->
+      P |- <((x <- a[[ie]], st, ast, b))> -->i_[DStep]^^[OARead a i]
+            <((skip, x !-> (nth i (ast a) 0); st, ast, b))>
+  | ISM_ARead_U : forall P x a ie st ast i a' i',
+      aeval st ie = i ->
+      P x = secret ->
+      i >= length (ast a) ->
+      i' < length (ast a') ->
+      P |- <((x <- a[[ie]], st, ast, true))> -->i_[DLoad a' i']^^[OARead a i]
+            <((skip, x !-> (nth i' (ast a') 0); st, ast, true))>
+  | ISM_Write : forall P a ie e st ast (b :bool) i n le,
+      aeval st e = n ->
+      P |-a- e \in le ->
+      (if negb le && b then 0 else (aeval st ie)) = i ->
+      i < length (ast a) ->
+      P |- <((a[ie] <- e, st, ast, b))> -->i_[DStep]^^[OAWrite a i]
+            <((skip, st, a !-> upd i (ast a) n; ast, b))>
+  | ISM_Write_U : forall P a ie e st ast i n a' i',
+      aeval st e = n ->
+      P |-a- e \in public ->
+      aeval st ie = i ->
+      i >= length (ast a) ->
+      i' < length (ast a') ->
+      P |- <((a[ie] <- e, st, ast, true))> -->i_[DStore a' i']^^[OAWrite a i]
+            <((skip, st, a' !-> upd i' (ast a') n; ast, true))>
+
+  where "P |- <(( c , st , ast , b ))> -->i_ ds ^^ os  <(( ct ,  stt , astt , bt ))>" :=
+    (ideal_eval_small_step P c st ast b ct stt astt bt ds os).
+
+Reserved Notation
+  "P '|-' '<((' c , st , ast , b '))>' '-->i*_' ds '^^' os '<((' ct , stt , astt , bt '))>'"
+  (at level 40, c custom com at level 99, ct custom com at level 99,
+   st constr, ast constr, stt constr, astt constr at next level).
+
+Inductive multi_ideal (P:pub_vars) (c:com) (st:state) (ast:astate) (b:bool) :
+    com -> state -> astate -> bool -> dirs -> obs -> Prop :=
+  | multi_ideal_refl : P |- <((c, st, ast, b))> -->i*_[]^^[] <((c, st, ast, b))>
+  | multi_ideal_trans (c':com) (st':state) (ast':astate) (b':bool)
+                (c'':com) (st'':state) (ast'':astate) (b'':bool)
+                (ds1 ds2 : dirs) (os1 os2 : obs) :
+      P |- <((c, st, ast, b))> -->i_ds1^^os1 <((c', st', ast', b'))> ->
+      P |- <((c', st', ast', b'))> -->i*_ds2^^os2 <((c'', st'', ast'', b''))> ->
+      P |- <((c, st, ast, b))> -->i*_(ds1++ds2)^^(os1++os2) <((c'', st'', ast'', b''))>
+
+  where "P |- <(( c , st , ast , b ))> -->i*_ ds ^^ os  <(( ct ,  stt , astt , bt ))>" :=
+    (multi_ideal P c st ast b ct stt astt bt ds os).
+
+Lemma multi_ideal_trans_nil_l P c st ast b c' st' ast' b' ct stt astt bt ds os :
+  P |- <((c, st, ast, b))> -->i_[]^^[] <((c', st', ast', b'))> ->
+  P |- <((c', st', ast', b'))> -->i*_ds^^os <((ct, stt, astt, bt))> ->
+  P |- <((c, st, ast, b))> -->i*_ds^^os <((ct, stt, astt, bt))>.
+Proof.
+  intros. rewrite <- app_nil_l. rewrite <- app_nil_l with (l:=ds). eapply multi_ideal_trans; eassumption.
+Qed.
+
+Lemma multi_ideal_trans_nil_r P c st ast b c' st' ast' b' ct stt astt bt ds os :
+  P |- <((c, st, ast, b))> -->i_ds^^os <((c', st', ast', b'))> ->
+  P |- <((c', st', ast', b'))> -->i*_[]^^[] <((ct, stt, astt, bt))> ->
+  P |- <((c, st, ast, b))> -->i*_ds^^os <((ct, stt, astt, bt))>.
+Proof.
+  intros. rewrite <- app_nil_r. rewrite <- app_nil_r with (l:=ds). eapply multi_ideal_trans; eassumption.
+Qed.
+
+Lemma multi_ideal_combined_executions :
+  forall P c st ast b ds cm stm astm bm osm dsm ct stt astt bt ost,
+    P |- <((c, st, ast, b))> -->i*_ds^^osm <((cm, stm, astm, bm))> ->
+    P |- <((cm, stm, astm, bm))> -->i*_dsm^^ost <((ct, stt, astt, bt))> ->
+    P |- <((c, st, ast, b))> -->i*_(ds++dsm)^^(osm++ost) <((ct, stt, astt, bt))>.
+Proof.
+  intros P c st ast b ds cm stm astm bm osm dsm ct stt astt bt ost Hev1 Hev2.
+  induction Hev1.
+  - do 2 rewrite app_nil_l. apply Hev2.
+  - do 2 rewrite <- app_assoc. eapply multi_ideal_trans.
+    + eapply H.
+    + apply IHHev1. apply Hev2.
+Qed.
+
+Lemma multi_ideal_add_snd_com : forall P c st ast ct stt astt ds os c2 b bt,
+  P |- <((c, st, ast, b))> -->i*_ds^^os <((ct, stt, astt, bt))> ->
+  P |- <((c;c2, st, ast, b))> -->i*_ds^^os <((ct;c2, stt, astt, bt))>.
+Proof.
+  intros. induction H; repeat econstructor; eauto.
+Qed.
+
+Conjecture addr_sel_slh_bcc : forall P c st ast (b:bool) ct stt astt bt ds os,
+  nonempty_arrs ast ->
+  unused "b" c ->
+  st "b" = (if b then 1 else 0) ->
+  <((addr_sel_slh P c, st, ast, b))> -->*_ds^^os <((ct, stt, astt, bt))> ->
+  exists c', P |- <((c, st, ast, b))> -->i*_ds^^os <((c', "b" !-> st "b"; stt, astt, bt))>.
+
+Conjecture gilles_lemma : forall P PA c st1 st2 ast1 ast2 ct1 ct2 stt1 stt2 astt1 astt2 ds os1 os2,
+  P ;; PA |-ct- c ->
+  pub_equiv P st1 st2 ->
+  P |- <((c, st1, ast1, true))> -->i*_ds^^os1 <((ct1, stt1, astt1, true))> ->
+  P |- <((c, st2, ast2, true))> -->i*_ds^^os2 <((ct2, stt2, astt2, true))> ->
+  os1 = os2.
+
+Conjecture ideal_eval_spec_ct_secure :
+  forall P PA c st1 st2 ast1 ast2 ct1 ct2 stt1 stt2 astt1 astt2 bt1 bt2 ds os1 os2,
+  P ;; PA |-ct- c ->
+  unused "b" c ->
+  st1 "b" = 0 ->
+  st2 "b" = 0 ->
+  pub_equiv P st1 st2 ->
+  pub_equiv PA ast1 ast2 ->
+  nonempty_arrs ast1 ->
+  nonempty_arrs ast2 ->
+  P |- <((c, st1, ast1, false))> -->i*_ds^^os1 <((ct1, stt1, astt1, bt1))> ->
+  P |- <((c, st2, ast2, false))> -->i*_ds^^os2 <((ct2, stt2, astt2, bt2))> ->
+  os1 = os2.
+
+Conjecture addr_sel_slh_spec_ct_secure :
+  forall P PA c st1 st2 ast1 ast2 ct1 ct2 stt1 stt2 astt1 astt2 bt1 bt2 ds os1 os2,
+  P ;; PA |-ct- c ->
+  unused "b" c ->
+  st1 "b" = 0 ->
+  st2 "b" = 0 ->
+  pub_equiv P st1 st2 ->
+  pub_equiv PA ast1 ast2 ->
+  nonempty_arrs ast1 ->
+  nonempty_arrs ast2 ->
+  <((addr_sel_slh P c, st1, ast1, false))> -->*_ds^^os1 <((ct1, stt1, astt1, bt1))> ->
+  <((addr_sel_slh P c, st2, ast2, false))> -->*_ds^^os2 <((ct2, stt2, astt2, bt2))> ->
+  os1 = os2.
